murec comp -> L comp

theories/L/Reductions/MuRec.v
@@ -417,6 +417,215 @@ Require Import Undecidability.L.Reductions.MuRec.MuRec_extract.
 
 Definition evalfun fuel c v := match eval fuel 0 c v with Some (inl x) => Some x | _ => None end.
 
+From Undecidability Require Import Compiler_spec MuRec_computable LVector.
+From Undecidability.TM Require Import NaryApp ClosedLAdmissible.
+
+Import L_Notations.
+
+Definition cont_vec (k : nat) : term := lam (many_lam k (k (Vector.fold_right (fun n s => (extT (@cons nat) (var n)) s) (many_vars k)  (ext (@nil nat))))).
+
+Lemma helper_closed k :
+  bound k (Vector.fold_right (fun (n : nat) (s0 : term) => extT (@cons nat) n s0) (many_vars k) (ext (@nil nat))).
+Proof.
+  induction k.
+  - cbn. cbv. repeat econstructor.
+  - rewrite many_vars_S. cbn. econstructor. econstructor. eapply closed_dcl_x. Lproc.
+    econstructor. lia.
+    eapply bound_ge. eauto. lia.
+Qed.
+
+Lemma subst_closed s n u :
+  closed s -> subst s n u = s.
+Proof.
+  now intros ->.
+Qed.
+
+Lemma vector_closed:
+  forall (k : nat) (v : Vector.t nat k) (x : term), Vector.In x (Vector.map enc v) -> proc x.
+Proof.
+  intros k v.
+  induction v; cbn; intros ? Hi. inversion Hi. inv Hi. Lproc. eapply IHv. eapply Eqdep_dec.inj_pair2_eq_dec in H2. subst. eauto. eapply nat_eq_dec.
+Qed.
+
+Lemma cont_vec_correct k s (v : Vector.t nat k) :
+  proc s ->
+  many_app (cont_vec k s) (Vector.map enc v) == s (enc v).
+Proof.
+  intros Hs.
+  unfold cont_vec.
+  rewrite equiv_many_app_L.
+  2:{ eapply beta_red. Lproc. rewrite subst_many_lam. replace (k + 0) with k by lia. reflexivity. }
+  cbn -[plus mult]. rewrite Nat.eqb_refl.
+  rewrite bound_closed_k. 2:eapply helper_closed.
+  replace (3 * k) with (k + 2 * k) by lia.
+  etransitivity.
+  eapply many_beta. eapply vector_closed.
+  rewrite many_subst_app.
+  rewrite many_subst_closed. 2:Lproc.
+  replace (2 * k) with (2 * k + 0) by lia.
+  eapply equiv_R.
+  induction v.
+  - cbn. reflexivity.
+  - rewrite many_vars_S. cbn -[mult]. rewrite subst_closed; [ | now Lproc].
+    rewrite Nat.eqb_refl.
+    rewrite !many_subst_app.
+    repeat (rewrite many_subst_closed; [ | now Lproc]).
+    rewrite bound_closed_k. 2:eapply helper_closed. rewrite IHv.
+    rewrite !enc_vector_eq.
+    change (extT (@cons nat)) with (ext (@cons nat)).
+    now Lsimpl.
+Qed.
+
+Definition mu_option : term := (lam (0 (mu (lam (1 0 (lam (enc true)) (enc false)))) (lam 0) (lam 0))).
+
+Lemma mu_option_proc : proc mu_option.
+Proof.
+  unfold mu_option. Lproc.
+Qed.
+#[export] Hint Resolve mu_option_proc : Lproc.
+
+From Undecidability Require Import LOptions.
+
+Lemma mu_option_equiv {X} `{registered X} s (b : X)  :
+  proc s ->
+  mu_option s == s (mu (lam (s 0 (lam (enc true)) (enc false)))) (lam 0) (lam 0).
+Proof.
+  unfold mu_option. intros Hs. now Lsimpl.
+Qed.
+
+Definition mu_option_spec {X} `{registered X} s (b : X)  :
+  proc s ->
+  (forall x : X, enc x <> lam 0) ->
+ (forall n : nat, exists o : option X, s (enc n) == enc o) ->
+  (forall b : X, forall m n : nat, s (enc n) == enc (Some b) -> m >= n -> s (enc m) == enc (Some b)) ->
+  mu_option s == enc b <-> exists n : nat, s (enc n) == enc (Some b).
+Proof.
+  intros Hs Hinv Ht Hm.
+  rewrite (@mu_option_equiv X); eauto.
+  split.
+  - intros He.
+    match goal with [He : ?s == _ |- _ ] => assert (converges s) as Hc end.
+    { eexists. split. exact He. Lproc. }
+    eapply app_converges in Hc as [Hc _].
+    eapply app_converges in Hc as [Hc _].
+    eapply app_converges in Hc as [_ Hc].
+    destruct Hc as [v [Hc Hv]].
+    pose proof (Hc' := Hc).
+    eapply mu_sound in Hc as [n [-> [Hc1 _]]]; eauto.
+    * exists n.
+      destruct (Ht n) as [ [x | ] Htt].
+      -- rewrite Htt.
+         enough (enc b == enc x) as -> % enc_extinj. reflexivity.
+         rewrite <- He.
+         rewrite Hc'. Lsimpl. rewrite Htt. now Lsimpl.
+      -- exfalso. eapply (Hinv b). eapply unique_normal_forms; try Lproc.
+         rewrite <- He, Hc'. Lsimpl.
+         rewrite Htt. Lsimpl. reflexivity.
+    * Lproc.
+    * intros n. destruct (Ht n) as [[] ];
+      eexists; Lsimpl; rewrite H0; Lsimpl; reflexivity.
+  - intros [n Hn].
+    edestruct mu_complete' with (n := n) as [n' [H' H'']].
+    4: rewrite H'.
+    + Lproc.
+    + intros m. destruct (Ht m) as [ [] ];
+      eexists; Lsimpl; rewrite H0; Lsimpl; reflexivity.
+    + Lsimpl. rewrite Hn. now Lsimpl.
+    + destruct (Ht n') as [[] Heq]; rewrite Heq; Lsimpl.
+      * enough (enc (Some x) == enc (Some b))by now eapply enc_extinj in H0; inv H0.
+        assert (n <= n' \/ n' <= n) as [Hl | Hl] by lia.
+        -- eapply Hm in Hl; eauto. now rewrite <- Heq, Hl.
+        -- eapply Hm in Hl; eauto. now rewrite <- Hn, Hl.
+      * enough (false = true) by congruence.
+        eapply enc_extinj. rewrite <- H''.
+        symmetry. Lsimpl. rewrite Heq. now Lsimpl.
+Qed.
+
+Instance computable_evalfun : computable evalfun.
+Proof. extract. Qed.
+
+Lemma vec_list_eq {n X} (v : Vector.t X n) :
+  vec_list v = Vector.to_list v.
+Proof.
+  induction v; cbn; f_equal; eassumption.
+Qed.  
+
+Lemma eval_mono c min k (v : Vector.t nat k) (f : recalg k) o :
+  eval c min (erase f) (vec_list v) = Some (inl o) -> forall c', c' >= c -> eval c' min (erase f) (vec_list v) = Some (inl o).
+Proof.
+  intros H c' Hl. eapply erase_correct in H.
+  eapply ra_bs_mono in H. 2: eauto.
+  now eapply erase_correct in H.
+Qed.
+
+Theorem computable_MuRec_to_L {k} (R : Vector.t nat k -> nat -> Prop) :
+  MuRec_computable R -> L_computable R.
+Proof.
+  intros [f Hf].
+  exists (cont_vec k (lam (mu_option (lam (ext evalfun 0 (enc (erase f)) 1))))).
+  intros v. rewrite <- many_app_eq_nat. split.
+  - intros m. rewrite L_facts.eval_iff.
+    assert (lambda (encNatL m)) as [b Hb]. { change  (lambda (enc m)). Lproc. }
+    rewrite Hb. rewrite eproc_equiv. rewrite cont_vec_correct. 2: unfold mu_option; Lproc.
+    assert (lam (mu_option (lam (ext evalfun 0 (enc (erase f)) 1))) (enc v) ==
+          mu_option (lam (ext evalfun 0 (enc (erase f)) (enc v)))).
+    {  unfold mu_option. now Lsimpl. }
+    rewrite H. rewrite <- Hb.
+    change (encNatL m) with (enc m).
+    rewrite mu_option_spec. 2:Lproc.
+    2:{ intros []; cbv; congruence. }
+    2:{ intros. eexists. rewrite !enc_vector_eq. Lsimpl. reflexivity. }
+    rewrite Hf.
+    split.
+    + intros [n Hn % erase_correct] % ra_bs_to_c. exists n.
+      rewrite !enc_vector_eq. Lsimpl.
+      unfold evalfun. rewrite <- vec_list_eq. now rewrite Hn.
+    + intros [n Hn]. eapply ra_bs_from_c. eapply erase_correct with (c := n).
+      match goal with [Hn : ?s == ?b |- _ ] => evar (t : term); assert (s == t) end.
+      rewrite !enc_vector_eq. Lsimpl. subst t. reflexivity. subst t.
+      rewrite vec_list_eq. rewrite H0 in Hn. eapply enc_extinj in Hn.
+      unfold evalfun in Hn. now destruct eval as [[] | ]; inv Hn.
+    + exact 0.
+    + intros. rewrite enc_vector_eq in *.
+      match type of H0 with ?s == ?b => evar (t : term); assert (s == t) end. Lsimpl. all: subst t. reflexivity. rewrite H2 in H0. clear H2.
+      eapply enc_extinj in H0. Lsimpl.
+      unfold evalfun in *.
+      destruct (eval n) as [ [] | ] eqn:E; inv H0.
+      rewrite <- vec_list_eq in *.
+      eapply eval_mono in E. rewrite E; eauto. lia.
+  - intros v' [H1 H2] % eval_iff.
+    eapply star_equiv_subrelation in H1.
+    rewrite cont_vec_correct in H1. 2: unfold mu_option; Lproc.
+    match goal with [Hn : ?s == ?b |- _ ] => evar (t : term); assert (s == t) end.
+    unfold mu_option. Lsimpl. all: subst t. reflexivity.
+    rewrite H in H1.
+    match type of H1 with ?s == _ => assert (converges s) end.
+    exists v'; split; eassumption.
+    eapply app_converges in H0 as [Hc _].
+    eapply app_converges in Hc as [Hc _].
+    eapply app_converges in Hc as [_ Hc].
+    destruct Hc as [v'' [Hc1 Hc2]].
+    pose proof (Hc1' := Hc1).
+    eapply mu_sound in Hc1; eauto.
+    + destruct Hc1 as [m [-> []]].
+      rewrite Hc1' in H1.
+      rewrite enc_vector_eq in H1.
+      destruct (evalfun m (erase f) (Vector.to_list v)) eqn:E.
+      * match type of H1 with ?s == ?b => evar (t : term); assert (s == t) end. Lsimpl. all: subst t. reflexivity.
+      rewrite H4, E in H1.
+      match type of H1 with ?s == ?b => evar (t : term); assert (s == t) end. Lsimpl. all: subst t. reflexivity.
+      rewrite H5 in H1.
+      eapply unique_normal_forms in H1. 2,3: Lproc.
+      subst. exists n. reflexivity.
+      * enough (true = false) by congruence. eapply enc_extinj.
+        rewrite <- H0. rewrite enc_vector_eq. Lsimpl.
+        now rewrite E.
+    + Lproc.
+    + intros n.
+      destruct (evalfun n (erase f) (Vector.to_list v)) eqn:EE;
+      eexists; rewrite enc_vector_eq; Lsimpl; rewrite EE; try Lsimpl; reflexivity.
+Qed.  
+
 Definition UMUREC_HALTING c := exists fuel, evalfun fuel c nil <> None.
 
 Import Undecidability.Synthetic.Definitions Undecidability.Synthetic.ReducibilityFacts.
@@ -449,4 +658,3 @@ Proof.
     + unfold evalfun in *. exists x0. destruct eval; try destruct s; try congruence.
     + exists x0. unfold evalfun in *. destruct eval; try destruct s; try congruence.
 Qed.
-(* Print Assumptions MUREC_WCBV. *)
