theories/MuRec/Util/MuRec_computable.v
@@ -3,6 +3,6 @@ From Undecidability.MuRec Require Import MuRec.
 From Coq Require Import List Vector Nat.
 Import ListNotations Vector.VectorNotations.
 
-Definition FRACTRAN_computable {k} (R : Vector.t nat k -> nat -> Prop) := 
+Definition MuRec_computable {k} (R : Vector.t nat k -> nat -> Prop) := 
   exists f : recalg k, forall v : Vector.t nat k, forall m : nat,
         forall m, R v m <-> ra_bs f v m.
